mc_reify/mccancel.v
@@ -2,8 +2,8 @@ Require Import MirrorCore.STac.STac.
 Require MirrorCore.syms.SymEnv.
 Require MirrorCore.syms.SymSum.
 Require Import MirrorCore.Lambda.ExprUnify_simul.
-Require Import MirrorCharge.OrderedCanceller.
-Require Import MirrorCharge.BILNormalize.
+(*Require Import MirrorCharge.OrderedCanceller.*)
+(*Require Import MirrorCharge.BILNormalize.*)
 Require Import MirrorCharge.SynSepLog.
 Require Import MirrorCharge.SepLogFold.
 Require Import MirrorCharge.ModularFunc.ILogicFunc.
@@ -12,8 +12,8 @@ Require Import Charge.Logics.ILogic.
 Require Import Charge.Logics.BILogic.
 Require Import MirrorCore.Subst.FMapSubst.
 Require Import MirrorCore.Lemma.
-Require Import MirrorCharge.ModularFunc.ReifyLemma.
-Require Import MirrorCharge.Java.Cancelation2.
+Require Import MirrorCharge.RTac.ReifyLemma.
+(*Require Import MirrorCharge.Java.Cancelation2.*)
 Require Export MirrorCore.RTac.RTac.
 Require Export MirrorCore.RTac.Core.
 Require Export MirrorCore.STac.STac.
@@ -23,18 +23,20 @@ Require Export types.
 Require Export funcs.
 Require Export reify.
 Require Import MirrorCore.Lambda.Expr.
-
+Require Import func_eq.
 
 Definition typeof_func_opt t := Some (typeof_func t).
 
 Global Instance RSym_Func' : SymI.RSym func' := {
    typeof_sym := typeof_func_opt;
    symD := funcD;
-   sym_eqb := fun a b => Some false
+   sym_eqb := fun a b => (Some (func_beq a b)) 
 }.
 
 Global Instance RSymOk_Func' : SymI.RSymOk RSym_Func'.
-Admitted.
+constructor.
+Admitted. (*guess we need complete equality??*)
+
 
 Instance ILogicOps_mpred : ILogicOps mpred := {
 lentails := derives;
@@ -124,7 +126,7 @@ Instance SS : SubstI.Subst subst (expr typ func) :=
   @FMapSubst.SUBST.Subst_subst _.
 Instance SU : SubstI.SubstUpdate subst (expr typ func) :=
   FMapSubst.SUBST.SubstUpdate_subst (@instantiate typ func).
-Instance SO : SubstI.SubstOk Expr_expr SS := 
+Instance SO : SubstI.SubstOk SS := 
   @FMapSubst.SUBST.SubstOk_subst typ RType_typ (expr typ func) _ _.
 
 Definition test_lemma :=
@@ -133,14 +135,14 @@ Definition test_lemma :=
           typrop
           (fun x => x) nil nil.
 
-Definition skip_lemma : lemma typ (expr typ func) (expr typ func).
+(*Definition skip_lemma : lemma typ (expr typ func) (expr typ func).
 reify_lemma reify_vst 
 @SeparationLogicSoundness.SoundSeparationLogic.CSL.semax_skip.
 Defined.
 
 Definition forward_setx_closed_now_lemma : lemma typ (expr typ func) (expr typ func).
 reify_lemma reify_vst forward_setx_closed_now.
-Defined.
+Defined.*)
 (*
 Goal forall (Espec : OracleKind) (Delta : tycontext) (Q : list (environ -> Prop))
    (R : list (environ -> mpred)) (id : ident) (e : Clight.expr)
@@ -175,7 +177,7 @@ Check forward_setx_closed_now.
 Print forward_setx_closed_now_lemma.
 Locate forward_setx_closed_now.
 *)
-
+(*
 Definition stac_cancel := @stac_cancel typ func subst tympred _ _ _ _ _ _ _ _.
 
 Definition fintro e : option (OpenAs typ (expr typ func)) :=
@@ -209,3 +211,4 @@ Definition cancel exp := (THEN (REPEAT 10 INTRO)
 (STAC_no_hyps (@ExprSubst.instantiate typ func) stac_cancel)) 
 CTop (SubstI.empty (expr := expr typ func)) exp.
 
+*)
